dependent state

secure_api/QuicProvider/quic_provider.c
@@ -15,7 +15,7 @@
 typedef struct quic_key {
   Crypto_AEAD_Invariant_aead_state st;
   Crypto_Indexing_id id;
-  char static_iv[12];
+  unsigned char static_iv[12];
 } quic_key;
 
 #if DEBUG
@@ -49,62 +49,62 @@ static void dump_secret(quic_secret *s)
   (a == TLS_hash_SHA256 ? Crypto_Hash_SHA256 : \
     (a == TLS_hash_SHA384 ? Crypto_Hash_SHA384 : Crypto_Hash_SHA512))
 
-int MITLS_CALLCONV quic_crypto_hash(quic_hash a, /*out*/ char *hash, const char *data, size_t len){
+int MITLS_CALLCONV quic_crypto_hash(quic_hash a, /*out*/ unsigned char *hash, const unsigned char *data, size_t len){
   if(a < TLS_hash_SHA256) return 0;
   Crypto_Hash_compute(CONVERT_ALG(a), len, (uint8_t*)data, (uint8_t*) hash);
   return 1;
 }
 
-int MITLS_CALLCONV quic_crypto_hmac(quic_hash a, char *mac,
-                     const char *key, uint32_t key_len,
-                     const char *data, uint32_t data_len) {
+int MITLS_CALLCONV quic_crypto_hmac(quic_hash a, unsigned char *mac,
+                     const unsigned char *key, uint32_t key_len,
+                     const unsigned char *data, uint32_t data_len) {
   if(a < TLS_hash_SHA256) return 0;
   Crypto_HMAC_compute(CONVERT_ALG(a), (uint8_t*) mac, (uint8_t*)key, key_len, (uint8_t*)data, data_len);
   return 1;
 }
 
-int MITLS_CALLCONV quic_crypto_hkdf_extract(quic_hash a, char *prk,
-                             const char *salt, uint32_t salt_len,
-                             const char *ikm, uint32_t ikm_len)
+int MITLS_CALLCONV quic_crypto_hkdf_extract(quic_hash a, unsigned char *prk,
+                             const unsigned char *salt, uint32_t salt_len,
+                             const unsigned char *ikm, uint32_t ikm_len)
 {
   if(a < TLS_hash_SHA256) return 0;
   Crypto_HKDF_hkdf_extract(CONVERT_ALG(a), (uint8_t*) prk, (uint8_t*)salt, salt_len, (uint8_t*)ikm, ikm_len);
   return 1;
 }
 
-int MITLS_CALLCONV quic_crypto_hkdf_expand(quic_hash a, char *okm, uint32_t olen, const char *prk, uint32_t prk_len, const char *info, uint32_t info_len)
+int MITLS_CALLCONV quic_crypto_hkdf_expand(quic_hash a, unsigned char *okm, uint32_t olen, const unsigned char *prk, uint32_t prk_len, const unsigned char *info, uint32_t info_len)
 {
   if(a < TLS_hash_SHA256) return 0;
   Crypto_HKDF_hkdf_expand(CONVERT_ALG(a), (uint8_t*) okm, (uint8_t*)prk, prk_len, (uint8_t*)info, info_len, olen);
   return 1;
 }
 
-int MITLS_CALLCONV quic_crypto_hkdf_tls_label(quic_hash a, char *info, size_t *info_len, const char *label)
+int MITLS_CALLCONV quic_crypto_hkdf_tls_label(quic_hash a, unsigned char *info, size_t *info_len, const char *label)
 {
   size_t label_len = strlen(label);
   uint32_t hlen = (a == TLS_hash_SHA256 ? 32 : (a == TLS_hash_SHA384 ? 48 : 64));
-  char *hash = alloca(hlen);
+  unsigned char *hash = alloca(hlen);
 
   if(a < TLS_hash_SHA256 || !info || !hash || label_len > 249)
     return 0;
 
   info[0] = 0;
-  info[1] = (char)hlen;
-  info[2] = (char)(label_len + 6);
+  info[1] = hlen;
+  info[2] = label_len + 6;
   memcpy(info+3, "tls13 ", 6);
   memcpy(info+9, label, label_len);
 
-  if(!quic_crypto_hash(a, hash, label, 0))
+  if(!quic_crypto_hash(a, hash, (const unsigned char*)label, 0))
     return 0;
 
-  info[9+label_len] = (char)hlen;
+  info[9+label_len] = hlen;
   memcpy(info + label_len + 10, hash, hlen);
   *info_len = label_len + 10 + hlen;
 
   return 1;
 }
 
-int MITLS_CALLCONV quic_crypto_hkdf_quic_label(quic_hash a, char *info, size_t *info_len, const char *label, uint16_t key_len)
+int MITLS_CALLCONV quic_crypto_hkdf_quic_label(quic_hash a, unsigned char *info, size_t *info_len, const char *label, uint16_t key_len)
 {
   uint32_t hlen = (a == TLS_hash_SHA256 ? 32 :
     (a == TLS_hash_SHA384 ? 48 : 64));
@@ -118,8 +118,7 @@ int MITLS_CALLCONV quic_crypto_hkdf_quic_label(quic_hash a, char *info, size_t *
   info[2] = (char)(label_len + 5);
   memcpy(info+3, "QUIC ", 5);
   memcpy(info+8, label, label_len);
-  info[8 + label_len] = 0;
-  *info_len = label_len + 9;
+  *info_len = label_len + 8;
 
   return 1;
 }
@@ -128,8 +127,8 @@ int MITLS_CALLCONV quic_crypto_tls_derive_secret(quic_secret *derived, const qui
 {
   uint32_t hlen = (secret->hash == TLS_hash_SHA256 ? 32 :
     (secret->hash == TLS_hash_SHA384 ? 48 : 64));
-  char *tmp = alloca(hlen);
-  char info[323] = {0};
+  unsigned char *tmp = alloca(hlen);
+  unsigned char info[323] = {0};
   size_t info_len;
 
   if(!quic_crypto_hkdf_tls_label(secret->hash, info, &info_len, label))
@@ -167,14 +166,15 @@ int MITLS_CALLCONV quic_crypto_tls_derive_secret(quic_secret *derived, const qui
   return 1;
 }
 
-int MITLS_CALLCONV quic_derive_handshake_secrets(quic_secret *client_hs, quic_secret *server_hs, const char *con_id, size_t con_id_len, const char *salt, size_t salt_len)
+int MITLS_CALLCONV quic_derive_handshake_secrets(quic_secret *client_hs, quic_secret *server_hs,
+   const unsigned char *con_id, size_t con_id_len, const unsigned char *salt, size_t salt_len)
 {
   quic_secret s0 = {
     .hash = TLS_hash_SHA256,
     .ae = TLS_aead_AES_128_GCM,
     .secret = {0}
   };
-  char info[259] = {0};
+  unsigned char info[259] = {0};
   size_t info_len;
 
   if(!quic_crypto_hkdf_extract(s0.hash, s0.secret, salt, salt_len, con_id, con_id_len))
@@ -182,15 +182,19 @@ int MITLS_CALLCONV quic_derive_handshake_secrets(quic_secret *client_hs, quic_se
 
   client_hs->hash = s0.hash;
   client_hs->ae = s0.ae;
+
   if(!quic_crypto_hkdf_quic_label(s0.hash, info, &info_len, "client hs", 32))
     return 0;
+
   if(!quic_crypto_hkdf_expand(s0.hash, client_hs->secret, 32, s0.secret, 32, info, info_len))
     return 0;
 
   server_hs->hash = s0.hash;
   server_hs->ae = s0.ae;
+
   if(!quic_crypto_hkdf_quic_label(s0.hash, info, &info_len, "server hs", 32))
     return 0;
+
   if(!quic_crypto_hkdf_expand(s0.hash, server_hs->secret, 32, s0.secret, 32, info, info_len))
     return 0;
 
@@ -202,14 +206,18 @@ int MITLS_CALLCONV quic_crypto_derive_key(quic_key **k, const quic_secret *secre
   quic_key *key = KRML_HOST_MALLOC(sizeof(quic_key));
   if(!key) return 0;
 
+#ifdef KRML_NOSTRUCT_PASSING
+  Crypto_Indexing_testId((Crypto_Indexing_aeadAlg)secret->ae, &key->id);
+#else
   key->id = Crypto_Indexing_testId((Crypto_Indexing_aeadAlg)secret->ae);
+#endif
 
   uint32_t klen = (secret->ae == TLS_aead_AES_128_GCM ? 16 : 32);
   uint32_t slen = (secret->hash == TLS_hash_SHA256 ? 32 :
     (secret->hash == TLS_hash_SHA384 ? 48 : 64));
 
-  char info[259] = {0};
-  char dkey[32];
+  unsigned char info[259] = {0};
+  unsigned char dkey[32];
   size_t info_len;
 
   if(!quic_crypto_hkdf_quic_label(secret->hash, info, &info_len, "key", klen))
@@ -227,36 +235,52 @@ int MITLS_CALLCONV quic_crypto_derive_key(quic_key **k, const quic_secret *secre
    printf("IV: "); dump(key->static_iv, 12);
 #endif
 
+#ifdef KRML_NOSTRUCT_PASSING
+  Crypto_AEAD_Main_coerce(&key->id, (uint8_t*)dkey, &key->st);
+#else
   key->st = Crypto_AEAD_Main_coerce(key->id, (uint8_t*)dkey);
+#endif
   *k = key;
   return 1;
 }
 
-static inline void sn_to_iv(char *iv, uint64_t sn)
+static inline void sn_to_iv(unsigned char *iv, uint64_t sn)
 {
   for(int i = 4; i < 12; i++)
     iv[i] ^= (sn >> (88-(i<<3))) & 255;
 }
 
-int MITLS_CALLCONV quic_crypto_create(quic_key **key, mitls_aead alg, const char *raw_key, const char *iv)
+int MITLS_CALLCONV quic_crypto_create(quic_key **key, mitls_aead alg, const unsigned char *raw_key, const unsigned char *iv)
 {
   quic_key *k = KRML_HOST_MALLOC(sizeof(quic_key));
   if(!k) return 0;
+#ifdef KRML_NOSTRUCT_PASSING
+  Crypto_Indexing_testId((Crypto_Indexing_aeadAlg)alg, &k->id);
+  Crypto_AEAD_Main_coerce(&k->id, (uint8_t*)raw_key, &k->st);
+#else
   k->id = Crypto_Indexing_testId((Crypto_Indexing_aeadAlg)alg);
   k->st = Crypto_AEAD_Main_coerce(k->id, (uint8_t*)raw_key);
+#endif
   memcpy(k->static_iv, iv, 12);
   *key = k;
   return 1;
 }
 
-int MITLS_CALLCONV quic_crypto_encrypt(quic_key *key, char *cipher, uint64_t sn, const char *ad, uint32_t ad_len, const char *plain, uint32_t plain_len)
+int MITLS_CALLCONV quic_crypto_encrypt(quic_key *key, unsigned char *cipher, uint64_t sn,
+  const unsigned char *ad, uint32_t ad_len, const unsigned char *plain, uint32_t plain_len)
 {
-  char iv[12];
+  unsigned char iv[12];
   memcpy(iv, key->static_iv, 12);
   sn_to_iv(iv, sn);
 
+#ifdef KRML_NOSTRUCT_PASSING
+  FStar_UInt128_t n;
+  Crypto_Symmetric_Bytes_load_uint128(12, (uint8_t*)iv, &n);
+  Crypto_AEAD_Main_encrypt(&key->id, &key->st, &n, ad_len, (uint8_t*)ad, plain_len, (uint8_t*)plain, (uint8_t*)cipher);
+#else
   FStar_UInt128_t n = Crypto_Symmetric_Bytes_load_uint128(12, (uint8_t*)iv);
   Crypto_AEAD_Main_encrypt(key->id, key->st, n, ad_len, (uint8_t*)ad, plain_len, (uint8_t*)plain, (uint8_t*)cipher);
+#endif
 
 #if DEBUG
   printf("ENCRYPT\nIV="); dump(iv, 12);
@@ -269,18 +293,26 @@ int MITLS_CALLCONV quic_crypto_encrypt(quic_key *key, char *cipher, uint64_t sn,
   return 1;
 }
 
-int MITLS_CALLCONV quic_crypto_decrypt(quic_key *key, char *plain, uint64_t sn, const char *ad, uint32_t ad_len, const char *cipher, uint32_t cipher_len)
+int MITLS_CALLCONV quic_crypto_decrypt(quic_key *key, unsigned char *plain, uint64_t sn,
+  const unsigned char *ad, uint32_t ad_len, const unsigned char *cipher, uint32_t cipher_len)
 {
-  char iv[12];
+  unsigned char iv[12];
   memcpy(iv, key->static_iv, 12);
   sn_to_iv(iv, sn);
 
   if(cipher_len < quic_crypto_tag_length(key))
     return 0;
 
+#ifdef KRML_NOSTRUCT_PASSING
+  FStar_UInt128_t n;
+  Crypto_Symmetric_Bytes_load_uint128(12, (uint8_t*)iv, &n);
+  uint32_t plain_len = cipher_len - quic_crypto_tag_length(key);
+  int r = Crypto_AEAD_Main_decrypt(&key->id, &key->st, &n, ad_len, (uint8_t*)ad, plain_len, (uint8_t*)plain, (uint8_t*)cipher);
+#else
   FStar_UInt128_t n = Crypto_Symmetric_Bytes_load_uint128(12, (uint8_t*)iv);
   uint32_t plain_len = cipher_len - quic_crypto_tag_length(key);
   int r = Crypto_AEAD_Main_decrypt(key->id, key->st, n, ad_len, (uint8_t*)ad, plain_len, (uint8_t*)plain, (uint8_t*)cipher);
+#endif
 
 #if DEBUG
   printf("DECRYPT %s\nIV=", r?"OK":"BAD"); dump(iv, 12);
